Share proof of `transfer` across languages

theories/Dot/typeExtractionSem.v
@@ -4,69 +4,7 @@ From D.Dot Require Import unary_lr typeExtractionSyn.
 
 Set Implicit Arguments.
 
-Implicit Types (T: ty) (v: vl) (e: tm) (Γ : ctx) (n: nat) (s: stamp).
-Notation sγmap := (gmap stamp gname).
-Implicit Types (g : stys) (sγ : sγmap).
-
-Section interp_equiv.
-  Context `{!dlangG Σ}.
-
-  Implicit Types (φ: envD Σ).
-
-  (* To give a definitive version of wellMapped, we need stampHeap to be stored in a resource. Here it is: *)
-  Definition wellMapped g : iProp Σ :=
-    (□∀ s T, ⌜ g !! s = Some T⌝ → s ↝ ⟦ T ⟧)%I.
-  Instance wellMapped_persistent g: Persistent (wellMapped g) := _.
-  Global Arguments wellMapped: simpl never.
-
-  (** We can transfer one mapping from [g] into Iris resources. *)
-  Lemma transferOne sγ g s T :
-    sγ !! s = None → allGs sγ ∧ wellMapped g ==∗
-    ∃ sγ', ⌜gdom sγ' ≡ {[s]} ∪ gdom sγ⌝ ∧ allGs sγ' ∧ wellMapped (<[s := T]> g).
-  Proof.
-    iIntros (HsFresh) "[Hallsγ #Hwmg]".
-    iMod (saved_ho_sem_type_alloc 0 (vopen (ty_interp T))) as (γ) "Hγ".
-    iMod (gen_iheap_alloc _ _ γ HsFresh with "Hallsγ") as "[Hallsγ Hs]".
-    iExists (<[s:=γ]> sγ); iModIntro; iFrame; iSplit. by rewrite dom_insert.
-    iAssert (s ↝ ⟦ T ⟧)%I as "#Hmaps {Hγ Hs}". iExists γ. by iFrame.
-    iIntros (s' T' Hlook) "!>". destruct (decide (s' = s)) as [->|Hne].
-    - suff ->: T' = T by []. move: Hlook. by rewrite lookup_insert => -[->].
-    - rewrite lookup_insert_ne // in Hlook. by iApply "Hwmg".
-  Qed.
-
-  Notation freshMappings g sγ := (∀ s, s ∈ gdom g → sγ !! s = None).
-
-  Lemma freshMappings_split s T g sγ :
-    freshMappings (<[s:=T]> g) sγ → sγ !! s = None ∧ freshMappings g sγ.
-  Proof.
-    intros Hdom; split => [|s' Hs']; apply Hdom;
-    rewrite dom_insert; set_solver.
-  Qed.
-
-  Lemma transfer' g sγ : freshMappings g sγ → allGs sγ ==∗
-    ∃ sγ', ⌜gdom sγ' ≡ gdom g ∪ gdom sγ⌝ ∧ allGs sγ' ∧ wellMapped g.
-  Proof.
-    elim g using map_ind.
-    - iIntros "/=" (H) "Hallsγ !>". iExists sγ; iFrame; iSplit.
-      + by rewrite dom_empty left_id.
-      + by iIntros (???).
-    - move => /= {g} s T g Hsg IH /freshMappings_split [Hssγ Hdom]. iIntros "Hallsγ".
-      iMod (IH Hdom with "Hallsγ") as (sγ' Hsγ') "Hown".
-      iMod (transferOne sγ' g s T with "Hown") as (sγ'' Hsγ'') "Hown".
-      + eapply (not_elem_of_dom (D := gset stamp)).
-        rewrite Hsγ' not_elem_of_union !not_elem_of_dom; by split.
-      + iExists sγ''; iFrame; iIntros "!%".
-        by rewrite Hsγ'' Hsγ' dom_insert union_assoc.
-  Qed.
-
-  Lemma transfer g sγ : freshMappings g sγ → allGs sγ ==∗ wellMapped g.
-  Proof.
-    iIntros (Hs) "H". by iMod (transfer' sγ Hs with "H") as (sγ' ?) "[_ $]".
-  Qed.
-
-  Lemma transfer_empty g : allGs ∅ ==∗ wellMapped g.
-  Proof. exact: transfer. Qed.
-End interp_equiv.
+Implicit Types (T: ty) (v: vl) (e: tm) (Γ : ctx) (n: nat) (s: stamp) (g : stys).
 
 Section typing_type_member_defs.
   Context `{!dlangG Σ}.
@@ -82,6 +20,7 @@ Section typing_type_member_defs.
   Arguments leadsto_envD_equiv /.
   Notation "s ↝[  σ  ] φ" := (leadsto_envD_equiv s σ φ) (at level 20).
 
+  Import stamp_transfer.
   Lemma extraction_to_leadsto_envD_equiv T g s σ n: T ~[ n ] (g, (s, σ)) →
     wellMapped g -∗ s ↝[ σ ] ty_interp T.
   Proof.
