theories/dlang.v
@@ -7,9 +7,10 @@ From D Require gen_iheap saved_interp_dep.
 
 Module mapsto.
 Export gen_iheap.
+Notation sγmap := (gmap stamp gname).
 
 Notation "s ↦ γ" := (mapsto (L := stamp) s γ) (at level 20) : bi_scope.
-Notation allGs gs := (gen_iheap_ctx (L := stamp) gs).
+Notation allGs sγ := (gen_iheap_ctx (L := stamp) sγ).
 
 Section mapsto_stamp_gname.
   Context `{gen_iheapG stamp gname Σ}.
@@ -189,4 +190,68 @@ Module Type LiftWp (Import VS : VlSortsSig).
       iApply (wp_wand with "Hwp"); by iIntros.
     Qed.
   End dlang_adequacy.
+
+  Module stamp_transfer.
+    Notation sγmap := (gmap stamp gname).
+
+    Notation gdom g := (dom (gset stamp) g).
+    Notation freshMappings g sγ := (∀ s, s ∈ gdom g → sγ !! s = None).
+
+    Section sec.
+      Context `{!dlangG Σ} `{!TyInterp ty Σ}.
+
+      Implicit Types (T: ty) (s: stamp) (g : gmap stamp ty) (sγ : sγmap).
+
+      Definition wellMapped g : iProp Σ :=
+        (□∀ s T, ⌜ g !! s = Some T⌝ → s ↝ ⟦ T ⟧)%I.
+      Instance wellMapped_persistent g: Persistent (wellMapped g) := _.
+      Global Arguments wellMapped: simpl never.
+
+      Lemma freshMappings_split s T g sγ :
+        freshMappings (<[s:=T]> g) sγ → sγ !! s = None ∧ freshMappings g sγ.
+      Proof.
+        intros Hdom; split => [|s' Hs']; apply Hdom;
+        rewrite dom_insert; set_solver.
+      Qed.
+
+      (** We can transfer one mapping from [g] into Iris resources. *)
+      Lemma transferOne sγ g s T :
+        sγ !! s = None → allGs sγ ∧ wellMapped g ==∗
+        ∃ sγ', ⌜gdom sγ' ≡ {[s]} ∪ gdom sγ⌝ ∧ allGs sγ' ∧ wellMapped (<[s := T]> g).
+      Proof.
+        iIntros (HsFresh) "[Hallsγ #Hwmg]".
+        iMod (saved_ho_sem_type_alloc 0 (vopen (ty_interp T))) as (γ) "Hγ".
+        iMod (gen_iheap_alloc _ _ γ HsFresh with "Hallsγ") as "[Hallsγ Hs]".
+        iExists (<[s:=γ]> sγ); iModIntro; iFrame; iSplit. by rewrite dom_insert.
+        iAssert (s ↝ ⟦ T ⟧)%I as "#Hmaps {Hγ Hs}". iExists γ. by iFrame.
+        iIntros (s' T' Hlook) "!>". destruct (decide (s' = s)) as [->|Hne].
+        - suff ->: T' = T by []. move: Hlook. by rewrite lookup_insert => -[->].
+        - rewrite lookup_insert_ne // in Hlook. by iApply "Hwmg".
+      Qed.
+
+      Lemma transfer' {g} sγ : freshMappings g sγ → allGs sγ ==∗
+        ∃ sγ', ⌜gdom sγ' ≡ gdom g ∪ gdom sγ⌝ ∧ allGs sγ' ∧ wellMapped g.
+      Proof.
+        elim g using map_ind.
+        - iIntros "/=" (H) "Hallsγ !>". iExists sγ; iFrame; iSplit.
+          + by rewrite dom_empty left_id.
+          + by iIntros (???).
+        - move => /= {g} s T g Hsg IH /freshMappings_split [Hssγ Hdom]. iIntros "Hallsγ".
+          iMod (IH Hdom with "Hallsγ") as (sγ' Hsγ') "Hown".
+          iMod (transferOne sγ' g s T with "Hown") as (sγ'' Hsγ'') "Hown".
+          + eapply (not_elem_of_dom (D := gset stamp)).
+            rewrite Hsγ' not_elem_of_union !not_elem_of_dom; by split.
+          + iExists sγ''; iFrame; iIntros "!%".
+            by rewrite Hsγ'' Hsγ' dom_insert union_assoc.
+      Qed.
+
+      Lemma transfer g sγ : freshMappings g sγ → allGs sγ ==∗ wellMapped g.
+      Proof.
+        iIntros (Hs) "H". by iMod (transfer' sγ Hs with "H") as (sγ' ?) "[_ $]".
+      Qed.
+
+      Lemma transfer_empty g : allGs ∅ ==∗ wellMapped g.
+      Proof. exact: transfer. Qed.
+    End sec.
+  End stamp_transfer.
 End LiftWp.
